fixed the 3rd problem in r3863: in the dominator relation a >> b, b can be phinodes.
The proofs w/o this were not wrong. In the existent proofs, we only
considered dominated commands and terminators. The well-formedness of
a phinode say that its incoming values must be dominated by the end of
the correspoinding incoming blocks. So, we never proved properties about
dominated phiniodes.

In mem2reg, we need to prove more lemmas about transitivity of
domination. In a>>b, a can be phinodes, so we need to consider dominated
phinodes.

All existent metatheory were extended for the change. We also proved
the acyclicness of idDominates and cmds_dominates_cmd that are needed by
id_rhs_val.



git-svn-id: https://webdav.seas.upenn.edu/svn/sol/vol@3866 eef5ea85-cc2e-0410-bd84-0fae1f012da8

src3.0/Vellvm/analysis.v
@@ -1044,13 +1044,24 @@ Definition inscope_of_block (f:fdef) (l1:l) (opt_ctx:option (list atom)) (lbl:l)
   | None => None
   end.
 
+Definition init_scope (f:fdef) (ps:phinodes) (cs:cmds) (id0:id) : list atom :=
+if (in_dec id_dec id0 (getPhiNodesIDs ps)) then
+  getArgsIDsOfFdef f
+else 
+  getPhiNodesIDs ps ++ cmds_dominates_cmd cs id0 ++ getArgsIDsOfFdef f.
+
 Definition inscope_of_id (f:fdef) (b1:block) (id0:id) : option (list atom) :=
 let '(block_intro l1 ps cs _) := b1 in
 let 'dt := dom_analyze f in
 let '(Dominators.mkBoundedSet els _) := AMap.get l1 dt in
-fold_left (inscope_of_block f l1) els
-  (Some (getPhiNodesIDs ps ++ cmds_dominates_cmd cs id0 ++ getArgsIDsOfFdef f))
+fold_left (inscope_of_block f l1) els (Some (init_scope f ps cs id0))
 .
+
+Definition value_in_scope (v0:value) (ids0:ids) : Prop :=
+match v0 with
+| value_const _ => True
+| value_id vid => In vid ids0
+end.
 
 Definition idDominates (f:fdef) (id1 id2: id) : Prop :=
 match lookupBlockViaIDFromFdef f id2 with
@@ -1060,6 +1071,14 @@ match lookupBlockViaIDFromFdef f id2 with
     | None => False
     end
 | None => False
+end.
+
+(* v1 >> v2 == id1 >> id2 \/ v1 is constant *)
+Definition valueDominates (f:fdef) (v1 v2:value) : Prop :=
+match v1, v2 with
+| value_id id1, value_id id2 => idDominates f id1 id2
+| value_const _, _ => True
+| _, _ => False
 end.
 
 Definition inscope_of_cmd (f:fdef) (b1:block) (c:cmd) : option (list atom) :=
@@ -1083,6 +1102,26 @@ match i with
 | insn_cmd c => inscope_of_cmd f curb c
 | insn_terminator tmn => inscope_of_tmn f curb tmn
 end.
+
+Lemma init_scope_spec1: forall f ps cs id0,
+  ~ In id0 (getPhiNodesIDs ps) ->
+  init_scope f ps cs id0 =
+    getPhiNodesIDs ps ++ cmds_dominates_cmd cs id0 ++ getArgsIDsOfFdef f.
+Proof.
+  intros.
+  unfold init_scope.
+  destruct_if; try tauto.
+Qed.
+
+Lemma init_scope_spec2: forall f ps cs id2 id1
+  (J1 : In id1 (init_scope f ps cs id2)) 
+  (Hnotin2 : ~ In id1 (getArgsIDsOfFdef f)),
+  In id1 (getPhiNodesIDs ps ++ cmds_dominates_cmd cs id2 ++ getArgsIDsOfFdef f).
+Proof.
+  unfold init_scope.
+  intros.
+  destruct_if; try tauto.
+Qed.
 
 Lemma getCmdsIDs__cmds_dominates_cmd : forall cs2' c',
   ~ In (getCmdLoc c') (getCmdsLocs cs2') ->
@@ -1205,8 +1244,8 @@ Proof.
       rewrite fold_left__none in H. inversion H.
 Qed.
 
-Lemma inscope_of_cmd_tmn : forall f l2 ps2 cs2' c' tmn' ids1,
-~ In (getCmdLoc c') (getCmdsLocs cs2') ->
+Lemma inscope_of_cmd_tmn : forall f l2 ps2 cs2' c' tmn' ids1
+(Huniq: NoDup (getBlockLocs (block_intro l2 ps2 (cs2'++[c']) tmn'))),
 Some ids1 = inscope_of_cmd f (block_intro l2 ps2 (cs2'++[c']) tmn') c' ->
 exists ids2,
   Some ids2 = inscope_of_tmn f (block_intro l2 ps2 (cs2'++[c']) tmn') tmn' /\
@@ -1215,18 +1254,30 @@ exists ids2,
   | None => set_eq _ ids1 ids2
   end.
 Proof.
-  intros f l2 ps2 cs2' c' tmn' ids1 Hnotin Hinscope.
-  unfold inscope_of_cmd, inscope_of_id in Hinscope.
+  intros f l2 ps2 cs2' c' tmn' ids1 Huniq Hinscope.
+  unfold inscope_of_cmd, inscope_of_id, init_scope in Hinscope.
+  assert (~ In (getCmdLoc c') (getCmdsLocs cs2') /\
+          ~ In (getCmdLoc c') (getPhiNodesIDs ps2)) as Hnotin.
+    simpl in Huniq. 
+    split.
+      split_NoDup.
+      solve_NoDup_notin.
+
+      eapply NoDup_disjoint; eauto.
+      apply in_or_app. left.
+      solve_in_list.    
+  destruct Hnotin as [Hnotin Hnotin'].
+  destruct_if; try tauto.
   unfold inscope_of_tmn.
   destruct f as [[f t i0 la va] bs].
   remember ((dom_analyze (fdef_intro (fheader_intro f t i0 la va) bs)) !! l2) as R.
   destruct R as [R_contents R_bound]. simpl in *.
   apply getCmdsIDs__cmds_dominates_cmd in Hnotin.
-  symmetry in Hinscope.
+  symmetry in H0.
   remember (getCmdID c') as R.
   destruct R.
-    apply fold_left__opt_union with (init2:=[i1]) in Hinscope.
-    destruct Hinscope as [r2 [Hinscope Heq]].
+    apply fold_left__opt_union with (init2:=[i1]) in H0.
+    destruct H0 as [r2 [Hinscope Heq]].
     apply fold_left__opt_set_eq with (init2:=((getPhiNodesIDs ps2) ++
       ((getCmdsIDs (cs2' ++ [c'])) ++ (getArgsIDs la)))) in Hinscope.
       destruct Hinscope as [r3 [Hinscope Heq']].
@@ -1248,8 +1299,8 @@ Proof.
           apply set_eq_sym; auto.
 
     apply fold_left__opt_set_eq with (init2:=((getPhiNodesIDs ps2) ++
-      ((getCmdsIDs (cs2' ++ [c'])) ++ (getArgsIDs la)))) in Hinscope.
-      destruct Hinscope as [r3 [Hinscope Heq']].
+      ((getCmdsIDs (cs2' ++ [c'])) ++ (getArgsIDs la)))) in H0.
+      destruct H0 as [r3 [Hinscope Heq']].
       exists r3.
       split; auto.
       apply set_eq_app; auto using set_eq_refl.
@@ -1296,10 +1347,10 @@ Proof.
        apply set_eq_app; auto using set_eq_refl.
 Qed.
 
-Lemma inscope_of_cmd_cmd : forall f l2 ps2 cs2' c' c cs' tmn' ids1,
-NoDup (getCmdsLocs (cs2'++[c']++[c]++cs')) ->
-Some ids1 = inscope_of_cmd f (block_intro l2 ps2 (cs2'++[c']++[c]++cs') tmn') c'
-  ->
+Lemma inscope_of_cmd_cmd : forall f l2 ps2 cs2' c' c cs' tmn' ids1
+(Huniq: NoDup (getBlockLocs (block_intro l2 ps2 (cs2'++[c']++[c]++cs') tmn')))
+(Hinscope: Some ids1 = 
+           inscope_of_cmd f (block_intro l2 ps2 (cs2'++[c']++[c]++cs') tmn') c'),
 exists ids2,
   Some ids2 =
     inscope_of_cmd f (block_intro l2 ps2 (cs2'++[c']++[c]++cs') tmn') c /\
@@ -1308,18 +1359,27 @@ exists ids2,
   | None => set_eq _ ids1 ids2
   end.
 Proof.
-  intros f l2 ps2 cs2' c' c cs' tmn' ids1 Hnodup Hinscope.
-  unfold inscope_of_cmd, inscope_of_id in Hinscope.
-  unfold inscope_of_cmd, inscope_of_id.
+  intros f l2 ps2 cs2' c' c cs' tmn' ids1 Huniq Hinscope.
+  unfold inscope_of_cmd, inscope_of_id, init_scope in Hinscope.
+  unfold inscope_of_cmd, inscope_of_id, init_scope.
+  assert (NoDup (getCmdsLocs (cs2'++[c']++[c]++cs'))) as Hnodup.
+    simpl in Huniq. split_NoDup. auto.
+  assert (~ In (getCmdLoc c) (getPhiNodesIDs ps2) /\
+          ~ In (getCmdLoc c') (getPhiNodesIDs ps2)) as Hnotin.
+    simpl in Huniq. 
+    split; eapply NoDup_disjoint; try solve 
+             [eauto | apply in_or_app; left; solve_in_list].
+  destruct_if; try tauto.
+  destruct_if; try tauto. clear Hnotin.
   destruct f as [[f t i0 la va] bs].
   remember ((dom_analyze (fdef_intro (fheader_intro f t i0 la va) bs)) !! l2) as R.
   destruct R as [R_contents R_bound].
   apply cmds_dominates_cmd__cmds_dominates_cmd in Hnodup. simpl in *.
-  symmetry in Hinscope.
+  symmetry in H0.
   remember (getCmdID c') as R.
   destruct R.
-    apply fold_left__opt_union with (init2:=[i1]) in Hinscope.
-    destruct Hinscope as [r2 [Hinscope Heq]].
+    apply fold_left__opt_union with (init2:=[i1]) in H0.
+    destruct H0 as [r2 [Hinscope Heq]].
     apply fold_left__opt_set_eq with (init2:=((getPhiNodesIDs ps2) ++
       ((cmds_dominates_cmd (cs2' ++ c' :: c :: cs') (getCmdLoc c)) ++
       (getArgsIDs la)))) in Hinscope.
@@ -1343,8 +1403,8 @@ Proof.
 
     apply fold_left__opt_set_eq with (init2:=((getPhiNodesIDs ps2) ++
       ((cmds_dominates_cmd (cs2' ++ c' :: c :: cs') (getCmdLoc c)) ++
-      (getArgsIDs la)))) in Hinscope.
-      destruct Hinscope as [r3 [Hinscope Heq']].
+      (getArgsIDs la)))) in H0.
+      destruct H0 as [r3 [Hinscope Heq']].
       exists r3.
       split; auto.
       apply set_eq_app; auto using set_eq_refl.
@@ -1482,10 +1542,7 @@ Proof.
   destruct insn2; tinv H.
     destruct H as [[ps1 [p1 [ps2 [J1 J2]]]] |
                    [cs1 [c1 [cs2 [cs3 [J1 J2]]]]]]; subst; simpl.
-      apply in_or_app.
-      left. rewrite getPhiNodesIDs_app.
-      apply in_or_app.
-      right. simpl. auto.
+      solve_in_list.
 
       apply in_or_app.
       right. apply InGetCmdsIDs_middle'; auto.
@@ -1495,8 +1552,7 @@ Proof.
       apply in_or_app.
       right. apply InGetCmdsIDs_middle'; auto.
 
-      apply in_or_app.
-      left. apply InGetPhiNodesIDs_middle; auto.
+      solve_in_list.
 Qed.
 
 Lemma insnDominates_spec3 : forall F b i0 insn2,
@@ -1582,61 +1638,6 @@ Proof.
       remember (getCmdID a) as R.
       destruct R; auto.
       rewrite IHcs; auto.
-Qed.
-
-Lemma insnDominates_trans: forall id1 p c t id2 l1 instr
-  (G : In id2 (getCmdsLocs c))
-  (H : In id1 (getPhiNodesIDs p ++ cmds_dominates_cmd c id2))
-  (H3 : NoDup (getBlockLocs (block_intro l1 p c t)))
-  (H1 : insnDominates id2 instr (block_intro l1 p c t)),
-  insnDominates id1 instr (block_intro l1 p c t).
-Proof.
-  intros.
-  apply in_app_or in H.
-  destruct H as [H | H]; simpl in *.
-    destruct instr; auto.
-      left. apply in_getPhiNodesIDs_inv; auto.
-
-      destruct H1 as [H1 Heq]; subst.
-      split; auto.
-      right. apply in_getPhiNodesIDs_inv; auto.
-
-    destruct instr; auto.
-      right.
-      destruct H1 as [[ps1 [p1 [ps2 [J1 J2]]]] |
-                      [cs1 [c1 [cs2 [cs3 [J1 J2]]]]]]; subst; simpl.
-        apply NoDup_disjoint with (i0:=getPhiNodeID p1) in H3; auto.
-          contradict H3.
-          rewrite getPhiNodesIDs_app.
-          apply in_or_app. right. simpl. auto.
-
-          apply in_or_app. left. auto.
-
-        apply NoDup_inv in H3. destruct H3 as [_ H3].
-        apply NoDup_inv in H3. destruct H3 as [H3 _].
-        rewrite cmds_dominates_cmd_spec3 in H; eauto using getCmdID__getCmdLoc.
-        apply in_getCmdsIDs_inv in H.
-        destruct H as [cs6 [c3 [cs7 [J6 J7]]]]; subst.
-        exists cs6. exists c3. exists (cs7 ++ c1 :: cs2). exists cs3.
-        simpl_env. split; auto.
-
-      destruct H1 as [[[cs1 [c1 [cs2 [J1 J2]]]] |
-                       [ps1 [p1 [ps2 [J1 J2]]]]] Heq]; subst; simpl.
-        apply NoDup_inv in H3. destruct H3 as [_ H3].
-        apply NoDup_inv in H3. destruct H3 as [H3 _].
-        rewrite cmds_dominates_cmd_spec3 in H; eauto using getCmdID__getCmdLoc.
-        apply in_getCmdsIDs_inv in H.
-        destruct H as [cs6 [c3 [cs7 [J6 J7]]]]; subst.
-        split; auto. left.
-        exists cs6. exists c3. exists (cs7 ++ c1 :: cs2).
-        simpl_env. split; auto.
-
-        apply NoDup_disjoint with (i0:=getPhiNodeID p1) in H3; auto.
-          contradict H3.
-          rewrite getPhiNodesIDs_app.
-          apply in_or_app. right. simpl. auto.
-
-          apply in_or_app. left. auto.
 Qed.
 
 Lemma insnDominates_spec1 : forall c1 block',
@@ -1844,6 +1845,9 @@ Proof.
   destruct HeqR0 as [J1 [J2 J3]].
   apply J3 in H.
   destruct H as [H | [b2 [l2 [H1 [H2 H3]]]]].
+    unfold init_scope in H.
+    simpl in H.
+    destruct_if; try tauto.
     exists (block_intro l1 p c t).
     symmetry in HeqR.
     apply lookupBlockViaIDFromFdef__blockInFdefB in HeqR.
@@ -1875,6 +1879,8 @@ Proof.
   destruct HeqR2 as [J1 [J2 J3]].
   apply J3 in Hdom.
   destruct Hdom as [Hdom | [b1 [l1' [H4 [H5 H6]]]]].
+    unfold init_scope in Hdom.
+    destruct_if; try tauto.
     right.
     apply lookupBlockViaIDFromFdef__blockInFdefB in H.
     apply block_eq1 with (b2:=block_intro l2 p0 c0 t0) in J; eauto.
@@ -1911,18 +1917,22 @@ Proof.
   destruct HeqR0 as [J1 [J2 J3]].
   apply J3 in H.
   destruct H as [H | [b2 [l2 [H1 [H2 H3]]]]].
-    symmetry in HeqR.
-    apply lookupBlockViaIDFromFdef__blockInFdefB in HeqR.
-    rewrite_env ((getPhiNodesIDs ps ++ cmds_dominates_cmd cs id2) 
-                   ++ getArgsIDs la) in H.
-    apply in_app_or in H.
-    destruct H as [H | H].
-      eapply inGetBlockLocs__lookupTypViaIDFromFdef in HeqR; eauto.
-      simpl. 
-      apply cmds_dominates_cmd_spec' in H.
-        solve_in_list.
+    unfold init_scope in H.
+    destruct_if.
+      eapply InArgsIDs_lookupTypViaIDFromFdef; eauto.
 
-        eapply InArgsIDs_lookupTypViaIDFromFdef; eauto.
+      symmetry in HeqR.
+      apply lookupBlockViaIDFromFdef__blockInFdefB in HeqR.
+      rewrite_env ((getPhiNodesIDs ps ++ cmds_dominates_cmd cs id2) 
+                   ++ getArgsIDs la) in H.
+      apply in_app_or in H.
+      destruct H as [H | H].
+        eapply inGetBlockLocs__lookupTypViaIDFromFdef in HeqR; eauto.
+        simpl. 
+        apply cmds_dominates_cmd_spec' in H.
+          solve_in_list.
+
+          eapply InArgsIDs_lookupTypViaIDFromFdef; eauto.
 
     apply lookupBlockViaLabelFromFdef__blockInFdefB in H2; auto.
     eapply inGetBlockLocs__lookupTypViaIDFromFdef in H2; eauto.
@@ -1942,49 +1952,97 @@ Proof.
   destruct b. eapply insnDominates_spec3 in H1; eauto.
 Qed.
 
+Lemma insnDominates_trans: forall id1 p c t id2 l1 instr f
+  (G : ~ In id1 (getArgsIDsOfFdef f))
+  (H : In id1 (init_scope f p c id2))
+  (H3 : NoDup (getBlockLocs (block_intro l1 p c t)))
+  (H1 : insnDominates id2 instr (block_intro l1 p c t)),
+  insnDominates id1 instr (block_intro l1 p c t).
+Proof.
+  intros.
+  unfold init_scope in H.
+  destruct_if; try tauto.
+  apply in_app_or in H.
+  destruct H as [H | H]; simpl in *.
+  Case "id1 in p".
+    destruct instr; auto.
+      left. apply in_getPhiNodesIDs_inv; auto.
+
+      destruct H1 as [H1 Heq]; subst.
+      split; auto.
+      right. apply in_getPhiNodesIDs_inv; auto.
+
+  apply in_app_or in H.
+  destruct H as [H | H]; simpl in *; try tauto.
+  Case "id1 in cs".
+    destruct instr; auto.
+    SCase "instr=cmd".
+      right.
+      destruct H1 as [[ps1 [p1 [ps2 [J1 J2]]]] |
+                      [cs1 [c1 [cs2 [cs3 [J1 J2]]]]]]; subst; simpl.
+      SSCase "p >> cmd".
+        clear HeqR. contradict n. solve_in_list.
+      SSCase "cmd >> cmd".
+        split_NoDup.
+        rewrite cmds_dominates_cmd_spec3 in H; eauto using getCmdID__getCmdLoc.
+        apply in_getCmdsIDs_inv in H.
+        destruct H as [cs6 [c3 [cs7 [J6 J7]]]]; subst.
+        exists cs6. exists c3. exists (cs7 ++ c1 :: cs2). exists cs3.
+        simpl_env. split; auto.
+
+    SCase "instr=tmn".
+      destruct H1 as [[[cs1 [c1 [cs2 [J1 J2]]]] |
+                       [ps1 [p1 [ps2 [J1 J2]]]]] Heq]; subst; simpl.
+      SSCase "cmd >> tmn".
+        split_NoDup.
+        rewrite cmds_dominates_cmd_spec3 in H; eauto using getCmdID__getCmdLoc.
+        apply in_getCmdsIDs_inv in H.
+        destruct H as [cs6 [c3 [cs7 [J6 J7]]]]; subst.
+        split; auto. left.
+        exists cs6. exists c3. exists (cs7 ++ c1 :: cs2).
+        simpl_env. split; auto.
+      SSCase "p >> tmn".
+        clear HeqR. contradict n. solve_in_list.
+Qed.
+
 Lemma idDominates_insnDominates__insnDominates : forall f id1 id2 b instr
   (Hnotin: ~ In id1 (getArgsIDsOfFdef f))
-  (G: exists c2, lookupInsnViaIDFromFdef f id2 = Some (insn_cmd c2)),
-  idDominates f id1 id2 ->
-  lookupBlockViaIDFromFdef f id1 = ret b ->
-  insnDominates id2 instr b ->
-  blockInFdefB b f = true ->
-  uniqFdef f ->
+  (H: idDominates f id1 id2)
+  (H0: lookupBlockViaIDFromFdef f id1 = ret b)
+  (H1: insnDominates id2 instr b)
+  (H2: blockInFdefB b f = true)
+  (H3: uniqFdef f),
   insnDominates id1 instr b.
 Proof.
   intros.
   unfold idDominates in H.
-  remember (lookupBlockViaIDFromFdef f id2) as R.
-  destruct R; tinv H.
-  remember (inscope_of_id f b0 id2) as R.
-  destruct R; tinv H.
-  unfold inscope_of_id in HeqR0.
-  destruct b0.
-  remember (Maps.AMap.get l1 (dom_analyze f)) as R.
+  inv_mbind. symmetry_ctx.
+  unfold inscope_of_id in *.
+  destruct b0 as [l1 p c t].
+  remember ( (dom_analyze f) !! l1) as R.
   destruct R.
-  symmetry in HeqR0. destruct f as [[fa ty fid la va] bs].
   apply fold_left__spec in HeqR0.
   destruct HeqR0 as [J1 [J2 J3]].
   apply J3 in H.
   destruct H as [H | [b2 [l2 [H1' [H2' H3']]]]].
-    symmetry in HeqR.
-    apply lookupBlockViaIDFromFdef__blockInFdefB in HeqR.
-    apply block_eq1 with (b2:=block_intro l1 p c t) in H0; eauto.
-      subst.
-      apply uniqFdef__uniqBlockLocs in H2; auto.
-      eapply insnDominates_trans; eauto.
-        apply insnDominates_spec4 in H1. simpl in H1.
-        eapply lookupCmdViaIDFromFdef_spec in HeqR; eauto.
-        solve_in_list.
+    assert (b = block_intro l1 p c t) as EQ.
+      eapply block_eq1 with (id0:=id1); eauto 1.
+        solve_blockInFdefB.
 
-        simpl in Hnotin. solve_in_list.
-
-      simpl.
-      eapply cmds_dominates_cmd_spec'' in H; eauto.
+        unfold init_scope in H.
+        destruct_if.
+          clear HeqR0.
+          contradict H. auto.
+          
+          simpl.
+          eapply cmds_dominates_cmd_spec''; eauto.
+    subst.  
+    eapply insnDominates_trans; eauto.
+      solve_NoDup.
 
     eapply insnDominates_spec3 in H1; eauto.
-    rewrite <- HeqR in H1. inv H1.
-    destruct b2.
+    uniq_result.
+    destruct b2 as [l3 p0 c0 t0].
     apply lookupBlockViaLabelFromFdef_inv in H2'; auto.
     destruct H2' as [Heq H2']; subst.
     apply block_eq1 with (b2:=block_intro l3 p0 c0 t0) in H0; auto.
@@ -1995,8 +2053,7 @@ Qed.
 
 Lemma idDominates_insnDominates__insnOrBlockStrictDominates :
 forall f id1 id2 b1 b instr
-  (Hnotin: ~ In id1 (getArgsIDsOfFdef f))
-  (G : exists c2, lookupInsnViaIDFromFdef f id2 = ret insn_cmd c2),
+  (Hnotin: ~ In id1 (getArgsIDsOfFdef f)),
   idDominates f id1 id2 ->
   lookupBlockViaIDFromFdef f id1 = ret b1 ->
   insnDominates id2 instr b ->
@@ -2039,10 +2096,10 @@ Lemma cmd_in_scope__block_in_scope: forall (l' : l) (F : fdef)
   (Heqdefs' : {| DomDS.L.bs_contents := contents';
                  DomDS.L.bs_bound := inbound' |} = (dom_analyze F) !! l')
   (Hinscope : fold_left (inscope_of_block F l') contents' (ret ids1) = ret ids0')
-  (id1 : atom) (Hid1 : In id1 ids0') (Hnotin' : ~ In id1 ids1) (c1 : cmd)
-  (Hlkc1 : lookupInsnViaIDFromFdef F id1 = ret insn_cmd c1)
+  (id1 : atom) (Hid1 : In id1 ids0') (Hnotin' : ~ In id1 ids1) insn1
+  (Hlkc1 : lookupInsnViaIDFromFdef F id1 = ret insn1)
   (l0 : l) (p : phinodes) (c : cmds) (t0 : terminator)
-  (H : insnInFdefBlockB (insn_cmd c1) F (block_intro l0 p c t0) = true),
+  (H : insnInFdefBlockB insn1 F (block_intro l0 p c t0) = true),
   In l0 contents'.
 Proof.
   intros. 
@@ -2057,11 +2114,11 @@ Proof.
   subst.
   eapply lookupBlockViaLabelFromFdef__lookupBlockViaIDFromFdef in J2;
     eauto.
-  eapply lookupInsnViaIDFromFdef_lookupBlockViaIDFromFdef__getCmdID in Hlkc1;
+  eapply lookupInsnViaIDFromFdef_lookupBlockViaIDFromFdef__getInsnID in Hlkc1;
     eauto.
   eapply insnInFdefBlockB__lookupBlockViaIDFromFdef in H; 
     try solve [eauto | congruence].
-  erewrite getCmdID__getCmdLoc in H; eauto.
+  erewrite getInsnID__getInsnLoc in H; eauto.
   uniq_result.
   apply ListSet.set_diff_elim1 in J1; auto.
 Qed.
@@ -2205,8 +2262,8 @@ Lemma cmds_dominates_cmd_inscope_of_cmd__inscope_of_cmd: forall
   (l2 : l) (p : phinodes) (c2 : cmds) (t0 : terminator)
   (HeqR1 : ret block_intro l2 p c2 t0 = lookupBlockViaIDFromFdef f id2)
   init (Heq: init = getArgsIDsOfFdef f)
-  (J1:In id1 (getPhiNodesIDs p ++ cmds_dominates_cmd c2 id2 ++ init))
-  (c0 : cmd) (HeqR0 : ret insn_cmd c0 = lookupInsnViaIDFromFdef f id2)
+  (J1:In id1 (init_scope f p c2 id2)) (Hnotin: ~ In id1 init)
+  instr0 (HeqR0 : ret instr0 = lookupInsnViaIDFromFdef f id2)
   (J12 : In id2
           (getPhiNodesIDs ps1 ++
            cmds_dominates_cmd (cs1 ++ c :: cs) (getCmdLoc c)))
@@ -2224,9 +2281,10 @@ Proof.
   inv EQ.
   apply fold_left__init in HeqR'.
   apply HeqR'; auto.
+    unfold init_scope in J1.
+    destruct_if; try tauto.
     eapply cmds_dominates_cmd_trans; eauto.
       apply cmds_dominates_cmd_spec' in J12.
-      eapply lookupCmdViaIDFromFdef_spec in HbInF; eauto.
       solve_in_list.
   
       apply uniqFdef__uniqBlockLocs in HbInF; auto.
@@ -2299,7 +2357,6 @@ Proof.
   rewrite <- HeqR3 in HeqR4. inv HeqR4.
   apply fold_left__intro with (l2:=l1')(B:=b1) in HeqR'; auto.
 Qed.
-
 
 Lemma cmds_dominates_cmd_inscope_of_tmn__inscope_of_tmn: forall
   (f : fdef) (t : list atom) (l1 : l) (ps1 : phinodes) (cs1 : cmds)
@@ -2402,14 +2459,64 @@ Qed.
 Lemma inscope_of_id__total: forall f b id0, inscope_of_id f b id0 <> None.
 Proof.
   unfold inscope_of_id. 
-  destruct f as [[fa ty fid la va] bs]. destruct b.
+  destruct f as [fh bs]. destruct b.
   intros. 
-  destruct ((dom_analyze (fdef_intro (fheader_intro fa ty fid la va) bs)) !! l0).
+  destruct ((dom_analyze (fdef_intro fh bs)) !! l0).
   eapply fold_left__bound_blocks 
-    with (fh:=fheader_intro fa ty fid la va)(l0:=l0)
-    (init:=getPhiNodesIDs p ++ cmds_dominates_cmd c id0 ++ getArgsIDs la) 
+    with (fh:=fh)(l0:=l0)(init:=init_scope (fdef_intro fh bs) p c id0) 
     in bs_bound; eauto.
   destruct bs_bound. simpl. congruence.
+Qed.
+
+Lemma inscope_of_cmd__idDominates : forall l0 f b c i0
+  (HeqR0 : ret l0 = inscope_of_cmd f b c) (Hin: In i0 l0) 
+  (Hsome: getCmdID c <> None) (Huniq: uniqFdef f)
+  (HbInF: blockInFdefB b f = true) (HcInB: cmdInBlockB c b = true),
+  idDominates f i0 (getCmdLoc c).
+Proof.
+  unfold inscope_of_cmd.
+  intros. 
+  eapply inscope_of_id__idDominates in HeqR0; eauto.
+  apply inGetBlockIDs__lookupBlockViaIDFromFdef; auto.
+    solve_in_list.
+Qed.
+          
+Lemma cmds_dominates_cmd_acyclic: forall (id1 id2 : id) (cs3 : cmds)
+  (Hnodup : NoDup (getCmdsLocs cs3))
+  (Hin2 : In id2 (cmds_dominates_cmd cs3 id1))
+  (Hin1 : In id1 (cmds_dominates_cmd cs3 id2))
+  (Hin3 : In id1 (getCmdsLocs cs3)) (Hin4 : In id2 (getCmdsLocs cs3)),
+  False.
+Proof.
+  intros.  
+  apply cmds_dominates_cmd_inv in Hin2; auto.
+  destruct Hin2 as [cs1 [c [cs2 [J1 [J2 J3]]]]]; subst.
+  apply cmds_dominates_cmd_inv in Hin1; auto.
+  destruct Hin1 as [cs1' [c' [cs2' [J1' [J2' J3']]]]]; subst.
+  apply in_getCmdsLocs_inv in J2.
+  destruct J2 as [cs4 [c1 [cs3 [G1 G2]]]]; subst.
+  apply in_getCmdsLocs_inv in J2'.
+  destruct J2' as [cs4' [c1' [cs3' [G1' G2']]]]; subst.
+  simpl_env in J1'. simpl_env in Hnodup. simpl in *.
+  assert (G:=Hnodup).
+  apply NoDup_getCmdsLocs_prop with (c1:=c1)(c2:=c') in G; 
+    try solve [auto | solve_in_list | rewrite J1'; solve_in_list].
+  subst.
+  assert (G:=Hnodup).
+  apply NoDup_getCmdsLocs_prop with (c1:=c1')(c2:=c) in G; 
+    try solve [auto | solve_in_list | rewrite J1'; solve_in_list].
+  subst.
+  rewrite_env ((cs4' ++ c :: cs3') ++ c' :: cs2') in J1'.
+  apply NoDup_cmds_split_middle in J1'; auto.
+  destruct J1'; subst.
+  clear - Hnodup.
+  simpl_env in Hnodup. 
+  rewrite getCmdsLocs_app in Hnodup.
+  apply NoDup_split in Hnodup. destruct Hnodup as [_ Hnodup].
+  rewrite getCmdsLocs_app in Hnodup.
+  simpl in Hnodup. inv Hnodup.
+  apply H1. rewrite_env ((cs3' ++ c' :: cs3) ++ c :: cs2).
+  solve_in_list.
 Qed.
 
 Inductive wf_phi_operands (f:fdef) (b:block) (id0:id) (t0:typ) :
