src3.0/Vellvm/opsem_wf.v
@@ -574,6 +574,11 @@ Proof.
       eapply wf_defs_br_aux; eauto.
 
   Case "cs'<>nil".
+    assert (~ In (getCmdLoc c) (getPhiNodesIDs ps')) as Hnotin.
+      apply uniqFdef__uniqBlockLocs in J; auto.
+      simpl in J. 
+      eapply NoDup_disjoint in J; simpl; eauto.
+    rewrite init_scope_spec1; auto.
     unfold cmds_dominates_cmd. simpl.
     destruct (eq_atom_dec (getCmdLoc c) (getCmdLoc c)) as [_ | n];
       try solve [contradict n; auto].
@@ -1643,19 +1648,11 @@ Proof.
       symmetry in Hid.
       apply getCmdLoc_getCmdID in Hid.
        subst.
+      assert (NoDup (getBlockLocs (block_intro l3 ps3 (cs3' ++ c0 :: cs) tmn))) 
+        as Hnotin.
+        eapply wf_system__uniq_block with (f:=F) in HwfSystem; eauto.
       destruct cs; simpl_env in *.
       Case "1.1.1".
-        assert (~ In (getCmdLoc c0) (getCmdsLocs cs3')) as Hnotin.
-          eapply wf_system__uniq_block with (f:=F) in HwfSystem; eauto.
-          simpl in HwfSystem.
-          apply NoDup_inv in HwfSystem.
-          destruct HwfSystem as [_ J].
-          apply NoDup_inv in J.
-          destruct J as [J _].
-          rewrite getCmdsLocs_app in J.
-          simpl in J.
-          apply NoDup_last_inv in J. auto.
-
         apply inscope_of_cmd_tmn in HeqR1; auto.
         destruct HeqR1 as [ids2 [J1 J2]].
         rewrite <- J1.
@@ -1669,13 +1666,6 @@ Proof.
           eapply uniqF__lookupTypViaIDFromFdef; eauto.
 
       Case "1.1.2".
-        assert (NoDup (getCmdsLocs (cs3' ++ [c0] ++ [c] ++ cs))) as Hnodup.
-          eapply wf_system__uniq_block with (f:=F) in HwfSystem; eauto.
-          simpl in HwfSystem.
-          apply NoDup_inv in HwfSystem.
-          destruct HwfSystem as [_ J].
-          apply NoDup_inv in J.
-          destruct J as [J _]. auto.
         apply inscope_of_cmd_cmd in HeqR1; auto.
         destruct HeqR1 as [ids2 [J1 J2]].
         rewrite <- J1.
@@ -1756,20 +1746,12 @@ Proof.
   repeat (split; try solve [auto]).
       Case "0".
       intros. congruence.
+      assert (NoDup (getBlockLocs (block_intro l3 ps3 (cs3' ++ c0 :: cs) tmn))) 
+        as Hnotin.
+        eapply wf_system__uniq_block with (f:=F) in HwfSystem; eauto.
       Case "1".
       destruct cs; simpl_env in *.
       SCase "1.1.1".
-        assert (~ In (getCmdLoc c0) (getCmdsLocs cs3')) as Hnotin.
-          eapply wf_system__uniq_block with (f:=F) in HwfSystem; eauto.
-          simpl in HwfSystem.
-          apply NoDup_inv in HwfSystem.
-          destruct HwfSystem as [_ J].
-          apply NoDup_inv in J.
-          destruct J as [J _].
-          rewrite getCmdsLocs_app in J.
-          simpl in J.
-          apply NoDup_last_inv in J. auto.
-
         apply inscope_of_cmd_tmn in HeqR1; auto.
         destruct HeqR1 as [ids2 [J1 J2]].
         rewrite <- J1.
@@ -1782,13 +1764,6 @@ Proof.
         eapply wf_defs_eq; eauto.
 
       SCase "1.1.2".
-        assert (NoDup (getCmdsLocs (cs3' ++ [c0] ++ [c] ++ cs))) as Hnodup.
-          eapply wf_system__uniq_block with (f:=F) in HwfSystem; eauto.
-          simpl in HwfSystem.
-          apply NoDup_inv in HwfSystem.
-          destruct HwfSystem as [_ J].
-          apply NoDup_inv in J.
-          destruct J as [J _]. auto.
         apply inscope_of_cmd_cmd in HeqR1; auto.
         destruct HeqR1 as [ids2 [J1 J2]].
         rewrite <- J1.
@@ -1905,19 +1880,13 @@ Case "sReturn".
 
     split.
     SSCase "1.1".
+      assert (NoDup (getBlockLocs 
+                       (block_intro l2 ps2
+                          (cs2' ++ insn_call i0 n c rt va v p :: cs') tmn'))) 
+        as Hnotin.
+        eapply wf_system__uniq_block with (f:=F') in HwfSystem; eauto.
       destruct cs'; simpl_env in *.
       SSSCase "1.1.1".
-        assert (~ In (getCmdLoc (insn_call i0 n c rt va v p)) 
-          (getCmdsLocs cs2')) as Hnotin.
-          eapply wf_system__uniq_block with (f:=F') in HwfSystem; eauto.
-          simpl in HwfSystem.
-          apply NoDup_inv in HwfSystem.
-          destruct HwfSystem as [_ J].
-          apply NoDup_inv in J.
-          destruct J as [J _].
-          rewrite getCmdsLocs_app in J.
-          simpl in J.
-          apply NoDup_last_inv in J. auto.
         apply inscope_of_cmd_tmn in HeqR2; auto.
         destruct HeqR2 as [ids2 [J1 J2]].
         rewrite <- J1.
@@ -1946,14 +1915,6 @@ Case "sReturn".
           eapply wf_defs_eq; eauto.
 
       SSSCase "1.1.2".
-        assert (NoDup (getCmdsLocs (cs2' ++ [insn_call i0 n c rt va v p] 
-          ++ [c0] ++ cs'))) as Hnodup.
-          eapply wf_system__uniq_block with (f:=F') in HwfSystem; eauto.
-          simpl in HwfSystem.
-          apply NoDup_inv in HwfSystem.
-          destruct HwfSystem as [_ J].
-          apply NoDup_inv in J.
-          destruct J as [J _]. auto.
         apply inscope_of_cmd_cmd in HeqR2; auto.
         destruct HeqR2 as [ids2 [J1 J2]].
         rewrite <- J1.
@@ -2015,18 +1976,12 @@ Case "sReturnVoid".
     split.
     SSCase "1.1".
       apply HwfCall' in HBinF1. simpl in HBinF1.
+      assert (NoDup (getBlockLocs 
+                       (block_intro l2 ps2 (cs2' ++ c' :: cs') tmn'))) 
+        as Hnotin.
+        eapply wf_system__uniq_block with (f:=F') in HwfSystem; eauto.
       destruct cs'; simpl_env in *.
       SSSCase "1.1.1".
-        assert (~ In (getCmdLoc c') (getCmdsLocs cs2')) as Hnotin.
-          eapply wf_system__uniq_block with (f:=F') in HwfSystem; eauto.
-          simpl in HwfSystem.
-          apply NoDup_inv in HwfSystem.
-          destruct HwfSystem as [_ J].
-          apply NoDup_inv in J.
-          destruct J as [J _].
-          rewrite getCmdsLocs_app in J.
-          simpl in J.
-          apply NoDup_last_inv in J. auto.
         clear - HeqR2 Hinscope2 H HwfCall' HBinF1 Hnotin H1.
         apply inscope_of_cmd_tmn in HeqR2; auto.
         destruct HeqR2 as [ids2 [J1 J2]].
@@ -2038,14 +1993,7 @@ Case "sReturnVoid".
         eapply wf_defs_eq; eauto.
 
       SSSCase "1.1.2".
-        assert (NoDup (getCmdsLocs (cs2' ++ [c'] ++ [c] ++ cs'))) as Hnodup.
-          eapply wf_system__uniq_block with (f:=F') in HwfSystem; eauto.
-          simpl in HwfSystem.
-          apply NoDup_inv in HwfSystem.
-          destruct HwfSystem as [_ J].
-          apply NoDup_inv in J.
-          destruct J as [J _]. auto.
-        clear - HeqR2 Hinscope2 H HwfCall' HBinF1 Hnodup H1.
+        clear - HeqR2 Hinscope2 H HwfCall' HBinF1 H1 Hnotin.
         apply inscope_of_cmd_cmd in HeqR2; auto.
         destruct HeqR2 as [ids2 [J1 J2]].
         rewrite <- J1.
@@ -2353,6 +2301,7 @@ Case "sCall".
        eapply preservation_dbCall_case; eauto using wf_params_spec.
 
        unfold inscope_of_cmd, inscope_of_id.
+       rewrite init_scope_spec1; auto.
        remember ((dom_analyze (fdef_intro (fheader_intro fa rt fid la va) lb))
          !! l') as R.
        destruct R. simpl. simpl in H2. subst.
